handle offset is now a Z rather than a N

theories/handle.v
@@ -1,11 +1,11 @@
 
-From Coq Require Import BinNat.
+From Coq Require Import ZArith.BinInt BinNat.
 From Wasm Require Export bytes.
 From mathcomp Require Import ssrbool ssrnat.
 
 Record handle : Type := {
     base : N;
-    offset : N;
+    offset : Z;
     bound : N;
     valid : bool;
     id : N;
@@ -14,7 +14,7 @@ Record handle : Type := {
 
 Definition dummy_handle :=
   {| base := N.zero ;
-    offset := N.zero ;
+    offset := Z.zero ;
     bound := N.zero ;
     valid := false ;
     id := N.zero |}.
@@ -27,7 +27,7 @@ Definition upd_handle_validity h b :=
     valid := h.(valid) && b |}.
 
 Definition slice_handle h n1 n2 :=
-  if N.leb N.zero n1 && N.ltb n1 h.(bound) && N.leb N.zero n2 then
+  if N.ltb n1 h.(bound) then
     Some {| base := h.(base) + n1 ;
            offset := h.(offset) ;
            bound := h.(bound) - n2 ;
@@ -35,7 +35,16 @@ Definition slice_handle h n1 n2 :=
            id := h.(id) |}
   else None.
 
+Definition handle_add h (n: Z) :=
+  {| base := h.(base) ;
+    offset := h.(offset) + n ;
+    bound := h.(bound) ;
+    valid := h.(valid) ;
+    id := h.(id) |}.
 
+
+Definition new_handle a n id :=
+  {| base := a ; offset := 0%Z ; bound := n ; valid := true ; id := id |}.
 
 Class HandleBytes : Type := {
     handle_size : N;
